lean4/Automaton/DFA/Examples.lean
@@ -9,18 +9,27 @@ import Mathlib.Data.Fin.Basic
 open Nat DFA
 
 
-def trans_fun : Fin 2 → Fin 2 → Fin 2
+def δ₁ : Fin 2 → Fin 2 → Fin 2
   | 0 , 1 => 1
   | 0 , 0 => 0
   | 1 , 1 => 1
   | 1 , 0 => 0
 
 -- accepts all words that end with '1'
-def last_is_one : DFA (Fin 2) := {q := Fin 2, init := 0 , fs := {1} , δ := trans_fun}
+def last_is_one : DFA (Fin 2) := {q := Fin 2, init := 0 , fs := {1} , δ := δ₁}
 
 def w₁ : word (Fin 2) := [ 1, 0 ]
 def w₂ : word (Fin 2) := [ 0 ,1 ]
 def w₃ : word (Fin 2) := [ ]
+
+theorem accepts_all_last_1 (w : word (Fin 2)) : dfa_accepts last_is_one (w ++ [1]) := by
+  apply accepts_suffix_if
+  intro q r
+  simp [last_is_one]
+  simp [last_is_one] at q
+  match q with
+  | 0 => simp
+  | 1 => simp
 
 
 #eval δ_star' last_is_one last_is_one.init w₁ -- 0
@@ -31,3 +40,25 @@ def w₃ : word (Fin 2) := [ ]
 
 #eval δ_star last_is_one w₃ -- 0
 #eval dfa_accepts last_is_one w₃ -- false
+
+-- accepts all words that start with 1
+def δ₂ : Fin 3 → Fin 2 → Fin 3
+  | 0 , 1 => 1
+  | 0 , 0 => 2
+  | 1 , 1 => 1
+  | 1 , 0 => 1
+  | _ , _ => 2
+
+def first_is_one : DFA (Fin 2) := {q := Fin 3, init := 0, fs := {1} , δ := δ₂}
+
+theorem accepts_all_first_1 (w : word (Fin 2)) : dfa_accepts first_is_one ([1] ++ w) := by
+  apply accepts_prefix_if
+  · simp
+  · intro q r
+    induction r with
+    | base => simp
+    | step qc rqc e s => simp [first_is_one] at s            
+                         rw [s]
+                         match e with
+                         | 0 => simp
+                         | 1 => simp
