lean4/Automaton/Finset/Basic.lean
@@ -1,5 +1,6 @@
 import Mathlib.Data.Finset.Basic
 import Mathlib.Data.Finset.Powerset
+import Mathlib.Data.FinEnum
 
 namespace Finset
 
@@ -24,5 +25,7 @@ def subtype_of_sset_subtype {α : Type _} {s ss : Finset α} (e : { x // x ∈ s
   intro iss
   exact ⟨ e.1 , by simp; apply Finset.mem_of_subset iss; exact e.2⟩ 
 
+
+def finenum_to_finset (α : Type _) [FinEnum α] : Finset α := ⟨ Multiset.ofList (FinEnum.toList α) , by apply FinEnum.nodup_toList⟩
 
 end Finset
